\section*{1. $(B \rightarrow C) \rightarrow (A \land B \rightarrow A \land C)$} 

\begin{flalign*}
&1.\quad (B \rightarrow C) & P \\
&2. \quad \qquad (A \land B) & P \\  
&3. \quad \qquad \qquad \lnot(A \land C) & \text{P para $(A \land C)$ Prova por absurdo} \\
&4. \quad \qquad \qquad \qquad B & 2, Simp \\
&5. \quad \qquad \qquad \qquad C & 1, 4 MP \\
&6. \quad \qquad \qquad \qquad A & 2, Simp \\
&7. \quad \qquad \qquad \qquad  A \land C & 5,6 Conj.\\
&8. \quad \qquad \qquad \qquad Falso & 3, 7 Contra.\\
&9. \quad \qquad (A \land C) & 3-8, PI\\
&10. \quad (A \land B \rightarrow A \land C) & 2, 9 PC\\
& \quad QED & 1, 10 P
\end{flalign*}

\[
\infer[\text{PC1: }(B \to C)]
  {(B \to C) \to (A \land B \to A \land C)}
  {
    \infer[\text{PC2: }(A \land B)]
      {A \land B \to A \land C}
      {
        \infer[\text{PI3: } \lnot (A \land C)]
          {A \land C}
          {
            \infer[\text{Simp.}]
              {B}
              {A \land B}
            &
            \infer[\text{MP}]
              {C}
              {B \to C & B}
            &
            \infer[\text{Simp.}]
              {A}
              {A \land B}
            &
            \infer[\text{Conj.}]
              {A \land C}
              {A & C}
            &
            \infer[\text{Contr.}]
              {Falso}
              {\lnot (A \land C) & (A \land C)}
          }
      }
  }
\]
