\subsection*{iv. Digamos que j√° tenhamos provado $A \rightarrow (B \rightarrow C)$. Mostre que $B \rightarrow (A \rightarrow C)$.} 

\begin{flalign*}
&1.\quad A \rightarrow (B \rightarrow C) & P \\
&2.\quad (A \rightarrow (B \rightarrow C)) \rightarrow (B \rightarrow (A \rightarrow (B \rightarrow C))) & A2 \\ 
&3.\quad B \rightarrow (A \rightarrow (B \rightarrow C)) &\text{1, 2, MP }\\
&4.\quad B \rightarrow [(A \rightarrow (B \rightarrow C)) \rightarrow ((A \rightarrow B) \rightarrow (A \rightarrow C))] & A2 \\
&5.\quad (B \rightarrow (A \rightarrow (B \rightarrow C))) \rightarrow (B \rightarrow ((A \rightarrow B) \rightarrow (A \rightarrow C))) & A2 \\
&6.\quad B \rightarrow ((A \rightarrow B) \rightarrow (A \rightarrow C)) &\text{3, 5 MP} \\
&7.\quad (B \rightarrow (A \rightarrow B)) \rightarrow (B \rightarrow (A \rightarrow C)) & A2 \\
&8.\quad \quad B & P \\
&9.\quad B \rightarrow (A \rightarrow B) & A1 \\
&10.\quad B \rightarrow (A \rightarrow C) & \text{7, 9, MP}\\
&11. QED
\end{flalign*}