\subsection*{iii. Digamos que jรก tenhamos provado os teoremas $A \rightarrow B$ e $B \rightarrow C$. Mostre que $A \rightarrow C$.} 

\begin{flalign*}
&1.\quad (A \rightarrow B) & P \\
&2.\quad (B \rightarrow C) & P \\ 
&3.\quad (B \rightarrow C) \rightarrow (A \rightarrow (B \rightarrow C)) & A1 \\
&4.\quad A \rightarrow (B \rightarrow C) & \text{2, 3, MP }\\
&5.\quad (A \rightarrow (B \rightarrow C)) \rightarrow ((A \rightarrow B) \rightarrow (A \rightarrow C)) & A2 \\
&6.\quad ((A \rightarrow B) \rightarrow (A \rightarrow C)) & \text{4, 5, MP }\\
&7.\quad A \rightarrow C & \text{1, 6, MP} \\
&8.\quad QED
\end{flalign*}