\section*{1. Prove que as fbfs a seguir estão corretas.}

\textbf{i) $\{par (a[i]) \land (i=j+1)\} \ a[j] := a[i] + 1 \{impar(a[i-1])\}$}

\begin{flalign*}
	 & 1. \quad \{impar(\text{se } i-1 = j \ \text{ então } \ a[i] + 1 \ \text{ senão } \ a[i-1])\} a[j] := a[i] + 1 \{impar(a[i-1])\} & AAA                      \\
	 & 2. \quad (par(a[i] \land (i=j+1))                                                                                               & P                        \\
	 & 3. \qquad i = j + 1                                                                                                             & \text{2 Simp}            \\
	 & 4. \qquad i - 1 = j                                                                                                             & T                        \\
	 & 5. \qquad (i-1 = j) \rightarrow (impar(a[i] + 1))                                                                               & \text{Pré-condição de 1} \\
	 & 6. \qquad par(a[i])                                                                                                             & \text{2 Simp}            \\
	 & 7. \qquad impar(a[i] + 1)                                                                                                       & \text{4,5 MP}            \\
	 & 8. \qquad impar(\text{se } i - 1 = j \ \text{ então } \ a[i] + 1 \ \text{senão} \ a[i-1])                                       & \text{4,5,7 T}           \\
	 & 9. \quad (par(a[i]) \land (i=j+1)) \rightarrow impar(\text{se } i - 1 = j \ \text{ então } \ a[i] + 1 \ \text{senão} \ a[i-1])  & \text{2-8 PC}            \\
	 & QED                                                                                                                             & \text{1,9 Conseq.}       \\
\end{flalign*}

\noindent \textbf{ii) $\{a[2] = 2 \land a[1] = 1\} \ a[a[2]] := 1 \ \{\exists z, (a[z] = 1) \land (a[2] = z)\}$}

\begin{flalign*}
	 & 1. \quad \{\exists z, (( \text{se } z = a[2] \ \text{ então } \ 1 \ \text{ senão } \ a[z]) = 1 \land (\text{se } 2 = a[2] \ \text{ então } \ 1 \ \text{ senão } \ a[2]) = z)\} a[a[2]] := 1 \{\exists z, (a[z] = 1 \land a[2] = z)\} & AAA                   \\
	 & 2. \quad (a[2] =  2 \land a[1] =  1)                                                                                                                                                                                                 & P                     \\
	 & 3. \qquad \quad a[2] = 2                                                                                                                                                                                                             & \text{2 Simp}         \\
	 & 4. \qquad \quad a[1] = 1                                                                                                                                                                                                             & \text{2, Simp}        \\
	 & 5. \qquad \quad (\text{se } 2 = a[2] \text{ então } \ 1 \ \text{ senão } \ a[2]) = 1                                                                                                                                                 & 3, T                  \\
	 & 6. \qquad \quad (\text{se } 1 = a[2] \ \text{ então } \ 1 \ \text{ senão } \ a[1]) = a[1]                                                                                                                                            & 3, T                  \\
	 & 7. \qquad \quad (\text{se } 1 = a[2] \ \text{ então } \ 1 \ \text{ senãoo } \ a[1]) = 1                                                                                                                                              & \text{4,6 T}          \\
	 & 8. \qquad \quad ((\text{se } 1 = a[2] \text{ então } 1 \text{ senão } a[1]) = 1 \land (\text{se } 2 = a[2] \text{ então } 1 \text{ senão } a[2]) = 1)                                                                                & 4, 5, \text{Conj}     \\
	 & 9 \qquad \quad \ \exists z, ((\text{se } z = a[2] \text{ então } 1 \text{ senão } a[z]) = 1 \land (\text{se } 2 = a[2] \text{ então } 1 \text{ senão } a[2]) = z)                                                                    & 8, T                  \\
	 & 10. \quad (a[2] = 2 \land a[1] = 1) \to \exists z, (( \text{se } z = a[2] \ \text{ então } \ 1 \ \text{ senão } \ a[z]) = 1 \land (\text{se } 2 = a[2] \ \text{ então } \ 1 \ \text{ senão } \ a[2]) = z)                            & \text{2-9 PC}         \\
	 & QED                                                                                                                                                                                                                                  & 1, 10, \text{Conseq.}
\end{flalign*}

